\section{Exercise 7}

Prove that $\vdash A \rightarrow B$ and $\vdash A$ imply that $\vdash B$.\\

\noindent
\textbf{Solution.} Instead of LK, we now use the sequent calculus from Definition 6 in the script.\\

\noindent
We show the following\footnote{$A, A \rightarrow B \vdash B$ is transformed into $\vdash A \wedge (A \rightarrow B) \rightarrow B$ by the deduction theorem.}: $\vdash A \wedge (A \rightarrow B) \rightarrow B$. By the definition of $\rightarrow$, this is equivalent to: $\vdash \neg A \vee (A \vee \neg B) \vee B$.\\

\noindent
\textbf{Sequent proof:}

$$
	\begin{array}{l l l}
		1. & \{A,\neg A, B\} & \mt{Axiom}\\
		2. & \{\neg A, \neg B, B\} & \mt{Axiom}\\
		3. & \{A \wedge \neg B, \neg A, B\} & \wedge\mt{-rule }\\
		4. & \{\neg A \vee (A \wedge \neg B), B\} & \vee\mt{-rule}\\
		5. & \{\neg A \vee (A \wedge \neg B) \vee B\} & \vee\mt{-rule}\\
	\end{array}
$$

Which was to be proven.

